shift-reset/core/tag.v
@@ -2,7 +2,10 @@ From Stdlib Require Import String.
 
 Record tag : Type := Tag { tag_car : string }.
 
-Definition tag_eq_dec : forall (tag1 tag2 : tag), {tag1 = tag2} + {tag1 <> tag2}.
+Lemma tag_eq_dec : forall (tag1 tag2 : tag), {tag1 = tag2} + {tag1 <> tag2}.
 Proof. decide equality; auto using string_dec. Defined.
 
-Definition tag_empty : tag := Tag "".
+Definition tag_eqb (tag1 tag2 : tag) : bool :=
+  eqb (tag_car tag1) (tag_car tag2).
+
+Definition tag_empty : tag := Tag EmptyString.
