shift-reset/core/var.v
@@ -2,5 +2,8 @@ From Stdlib Require Import String.
 
 Record var : Type := Var { var_car : string }.
 
-Definition var_eq_dec : forall (x1 x2 : var), {x1 = x2} + {x1 <> x2}.
+Lemma var_eq_dec : forall (x1 x2 : var), {x1 = x2} + {x1 <> x2}.
 Proof. decide equality; auto using string_dec. Defined.
+
+Definition var_eqb (x1 x2 : var) : bool :=
+  eqb (var_car x1) (var_car x2).
